Add liveness back; sharpen true-liveness.
True liveness was in fact no true liveness: This change allows
variables to remain dead if they are only used to compute values of
dead variables. Correctness requires an refinement relation and makes
only sense in the context of dead variable elimination:
If dead variables remain in the program, a dead computations may read
garbage from dead variables and get stuck.

Liveness.v
@@ -104,7 +104,7 @@ Qed.
 Inductive live_sound : list (live*params) -> stmt -> ann live -> Prop :=
 | LOpr x Lv b lv e (al:ann live)
   :  live_sound Lv b al
-  -> (Exp.freeVars e) ⊆ lv
+  -> live_exp_sound e lv
   -> (getAnn al\{{x}}) ⊆ lv
   -> live_sound Lv (stmtExp x e b) (annExp lv al)
 | LIf Lv x b1 b2 lv (al1 al2:ann live)
@@ -146,7 +146,7 @@ Proof.
   general induction s; destruct slv; try isabsurd.
   + edestruct IHs; eauto; try inv an; eauto;
     destruct_prop (getAnn slv\{{x}} ⊆ a);
-    destruct_prop (freeVars e ⊆ a); try dec_solve. 
+    destruct_prop (live_exp_sound e a); try dec_solve.
   + edestruct IHs1; try inv an; eauto;
     edestruct IHs2; try inv an; eauto;
     destruct_prop (x ∈ a); 
@@ -185,29 +185,12 @@ Lemma freeVars_live s lv Lv
 Proof.
   intros. general induction H; simpl; eauto. 
   + cset_tac; intuition. eapply H1. cset_tac; eauto. 
+    eapply freeVars_live; eauto.
   + cset_tac; intuition. rewrite H5; eauto. 
   + cset_tac; eauto.
   + eapply union_subset_3.
     rewrite IHlive_sound1; eauto.
     rewrite IHlive_sound2; eauto.
-Qed.
-
-
-Fixpoint live_rename (ϱ:env var) (an:ann live) : ann live :=
-  match an with
-    | annExp a an => annExp (lookup_set ϱ a) (live_rename ϱ an)
-    | annIf a ans ant => 
-      annIf (lookup_set ϱ a) (live_rename ϱ ans) (live_rename ϱ ant)
-    | annGoto a => annGoto (lookup_set ϱ a)
-    | annReturn a => annReturn (lookup_set ϱ a)
-    | annLet a ans ant => 
-      annLet (lookup_set ϱ a) (live_rename ϱ ans) (live_rename ϱ ant)
-  end.
-
-Lemma getAnn_live_rename ϱ al
-: getAnn (live_rename ϱ al) = lookup_set ϱ (getAnn al).
-Proof.
-  destruct al; eauto.
 Qed.
 
 Definition live_rename_L_entry (ϱ:env var) (x:live * params)
@@ -218,20 +201,25 @@ Definition live_rename_L (ϱ:env var) DL
 
 Lemma live_rename_sound DL s an (ϱ:env var)
 : live_sound DL s an 
-  -> live_sound (live_rename_L ϱ DL) (rename ϱ s) (live_rename ϱ an).
+  -> live_sound (live_rename_L ϱ DL) (rename ϱ s) (mapAnn (lookup_set ϱ) an).
 Proof.
   intros. general induction H; simpl.
-  + econstructor; eauto. rewrite rename_exp_freeVars; eauto.
-    eapply lookup_set_incl; eauto. intuition. intuition.
-    rewrite getAnn_live_rename. 
+  + econstructor; eauto.
+    eapply live_exp_sound_incl. Focus 2.
+    eapply Exp.live_freeVars. 
+    eapply Subset_trans.
+    eapply rename_exp_freeVars; eauto. intuition.
+    eapply lookup_set_incl; eauto. intuition. 
+    eapply Exp.freeVars_live; eauto.
+    rewrite getAnn_mapAnn. 
     cset_tac; eqs; simpl; eauto. eapply lookup_set_incl; eauto. intuition.
     eapply lookup_set_spec; eauto. intuition. 
     eapply lookup_set_spec in H3; eauto. destruct H3; dcr; eauto.
     eexists x0; intuition. cset_tac; eauto. intro. eapply H2. 
     rewrite <- H3; eauto. intuition.
   + econstructor; eauto. eapply lookup_set_spec; eauto. intuition.
-    rewrite getAnn_live_rename. eapply lookup_set_incl; eauto. intuition.
-    rewrite getAnn_live_rename. eapply lookup_set_incl; eauto. intuition.
+    rewrite getAnn_mapAnn. eapply lookup_set_incl; eauto. intuition.
+    rewrite getAnn_mapAnn. eapply lookup_set_incl; eauto. intuition.
   + pose proof (map_get_1 (live_rename_L_entry ϱ) H). 
     econstructor; eauto. rewrite of_list_lookup_list. 
     simpl. eapply Subset_trans. eapply lookup_set_minus_incl. intuition.
@@ -239,7 +227,7 @@ Proof.
     repeat rewrite lookup_list_length; eauto.
     rewrite of_list_lookup_list; try eapply lookup_set_incl; intuition.
   + econstructor. eapply lookup_set_spec. intuition. eexists; intuition; eauto.
-  + econstructor; eauto; try rewrite getAnn_live_rename.
+  + econstructor; eauto; try rewrite getAnn_mapAnn.
     eapply IHlive_sound1. eapply IHlive_sound2.
     rewrite of_list_lookup_list. eapply lookup_set_incl; eauto. intuition.
     intuition.
@@ -252,7 +240,7 @@ Qed.
 Inductive true_live_sound : list (live*params) -> stmt -> ann live -> Prop :=
 | TLOpr x Lv b lv e (al:ann live)
   :  true_live_sound Lv b al
-  -> (Exp.freeVars e) ⊆ lv
+  -> (x ∈ getAnn al -> live_exp_sound e lv)
   -> (getAnn al\{{x}}) ⊆ lv
   -> true_live_sound Lv (stmtExp x e b) (annExp lv al)
 | TLIf Lv x b1 b2 lv (al1 al2:ann live)
@@ -285,7 +273,7 @@ Proof.
   general induction s; destruct slv; try isabsurd.
   + edestruct IHs; eauto; try inv an; eauto;
     destruct_prop (getAnn slv\{{x}} ⊆ a);
-    destruct_prop (freeVars e ⊆ a); try dec_solve. 
+    destruct_prop (x ∈ getAnn slv -> live_exp_sound e a); try dec_solve. 
   + edestruct IHs1; try inv an; eauto;
     edestruct IHs2; try inv an; eauto;
     destruct_prop (x ∈ a); 
@@ -423,7 +411,8 @@ Proof.
   eapply IHLA; eauto.
   eapply agree_on_incl; eauto. eapply freeVars_live; eauto.
 Qed.
-
+(*
+We are going to prove a simapx result about dve instead.
 Inductive approxI 
   : list (live*params) -> I.block -> I.block -> Prop :=
   approxII DL Z s lv
@@ -438,19 +427,29 @@ Inductive liveSimI : I.state -> I.state -> Prop :=
   (AG:agree_on (getAnn lv) E E')
   : liveSimI (L, E, s) (L, E', s).
 
+Require Import SimApx.
+
 Lemma liveSimI_sim σ1 σ2
-  : liveSimI σ1 σ2 -> sim σ1 σ2.
+  : liveSimI σ1 σ2 -> simapx σ1 σ2.
 Proof.
   revert σ1 σ2. cofix; intros. 
   destruct H; inv LS; simpl; simpl in *; 
           try params_match_tac.
   + case_eq (exp_eval E e); intros.
-    eapply simS; try eapply plusO.
-    econstructor; eauto. econstructor; eauto.
-    instantiate (1:=v). erewrite <- exp_eval_live; eauto. 
-    eapply live_exp_sound_incl; try eapply live_freeVars. cset_tac; eauto.
+    destruct_prop(x ∈ getAnn al).
+    eapply simS; try eapply plusO. 
+    econstructor; eauto.     econstructor; eauto.
+    instantiate (1:=v). erewrite <- exp_eval_live; eauto.
     eapply liveSimI_sim. econstructor; eauto.
     eapply agree_on_update_same; eauto using agree_on_incl.
+    case_eq (exp_eval E' e); intros.
+    eapply simS; try eapply plusO. 
+    econstructor; eauto.     econstructor; eauto.
+    eapply liveSimI_sim. econstructor; eauto.
+    assert (getAnn al [=] getAnn al \ {{x}}). 
+    split; cset_tac; intuition. rewrite H5.
+    eapply agree_on_update_dead_both. cset_tac; intuition. 
+    eapply agree_on_incl; eauto.
     eapply simE; try eapply star_refl; eauto; stuck.
     erewrite <- exp_eval_live in def; eauto. congruence.
     eapply live_exp_sound_incl;try eapply live_freeVars; eauto.
@@ -537,7 +536,7 @@ Proof.
     econstructor; eauto using agree_on_incl. 
     eapply agree_on_incl; eauto.
 Qed.
-
+*)
 (* 
 *** Local Variables: ***
 *** coq-load-path: (("." "Lyn")) ***
